theories/logic/sem_sig.v
@@ -153,6 +153,32 @@ Qed.
 Notation "'μ∀TS:' θ , α , τ ⇒ κ | m " := (sem_sig_eff_rec m (λ θ α, τ%T) (λ θ α, κ%T))
   (at level 100, m, τ, κ at level 200) : sem_sig_scope.
 
+
+Definition sem_sig_os {Σ} (σ : sem_sig Σ) : sem_sig Σ := (σ.1, upcl OS σ.2).
+Notation "¡ σ" := (sem_sig_os σ) (at level 10) : sem_sig_scope.
+
+(* One-Shot Signatures *)
+
+Definition mono_iEff {Σ} (Ψ : iEff Σ) : iProp Σ :=
+    □ (∀ v Φ Φ', (∀ w, Φ w -∗ Φ' w) -∗ Ψ.(iEff_car) v Φ -∗ Ψ.(iEff_car) v Φ').
+
+Class IsOS {Σ} (σ : sem_sig Σ) := {
+    is_os :> MonoProt σ.2
+}.
+
+Global Instance bot_is_os {Σ} : IsOS (⊥ : sem_sig Σ).
+Proof. do 2 constructor. iIntros (v Φ Φ') "Himp []". Qed.
+
+Global Instance sem_rec_eff_os_is_os {Σ} (A B : sem_sig Σ → sem_ty Σ → sem_ty Σ) `{ NonExpansive2 A, NonExpansive2 B} : 
+  IsOS (μ∀TS: θ, α, A θ α ⇒ B θ α | OS)%S.
+Proof. 
+  constructor.
+  by apply sem_sig_eff_rec_mono_prot.
+Qed.
+  
+Global Instance os_is_os {Σ} (σ : sem_sig Σ) : IsOS (¡ σ)%S.
+Proof. constructor. apply upcl_mono_prot. Qed.
+
 (* Sub-Typing on Signatures *)
 
 Lemma sig_le_refl {Σ} (σ : sem_sig Σ) : ⊢ σ ≤S σ.
@@ -201,4 +227,23 @@ Proof.
   - iDestruct "HκΦ₁" as "#HκΦ₁".
     iIntros "!# %b Hκ₂". iApply "HκΦ₁".
     iNext. iApply ("Hκ₂₁" with "IH Hκ₂").
+Qed.
+
+Lemma sig_le_os {Σ} (σ : sem_sig Σ) `{! IsOS σ} :
+  ⊢ ¡ σ ≤S σ.
+Proof.
+  iRight. rewrite /sem_sig_os. iSplit.
+  { iPureIntro. by destruct σ.1. }
+  iIntros (v Φ) "!# (%Φ' & Hσ & Himp)". simpl.
+  destruct IsOS0 as [[]].
+  iApply (monotonic_prot v Φ' Φ with "Himp Hσ"). 
+Qed.
+  
+Lemma sig_le_os_inv {Σ} (σ : sem_sig Σ) :
+  ⊢ σ ≤S (¡ σ).
+Proof.
+  iRight. rewrite /sem_sig_os. iSplit.
+  { iPureIntro. by destruct σ.1. }
+  iIntros (v Φ) "!# Hσ". simpl.
+  iExists Φ. iFrame. iIntros "% $".
 Qed.
