theories/case_studies/state.v
@@ -16,14 +16,16 @@ From haffel.lib Require Import base.
 From haffel.lang Require Import hazel.
 From haffel.logic Require Import sem_def.
 From haffel.logic Require Import sem_env.
+From haffel.logic Require Import sem_sig.
 From haffel.logic Require Import sem_types.
+From haffel.logic Require Import sem_judgement.
 From haffel.logic Require Import sem_sub_typing.
 From haffel.logic Require Import sem_operators.
 From haffel.logic Require Import compatibility.
 From haffel.logic Require Import tactics.
 
-Definition get : val := (λ: <>, perform: (InjL #()))%V.
-Definition put : val := (λ: "s", (perform: InjR "s") ;; #())%V.
+Definition get : val := (λ: <>, performₘ: (InjL #()))%V.
+Definition put : val := (λ: "s", (performₘ: InjR "s") ;; #())%V.
 
 Definition fact : val :=
   (rec: "fact" "n" := if: #1 < "n" then put (get #() * "n");; "fact" ("n" - #1)
@@ -86,7 +88,10 @@ Section typing.
     ⊢ ⊨ᵥ fact : (ℤ -{ stsig }-> ()).
   Proof.
     iIntros. iApply sem_typed_closure; solve_sidecond.
-    simpl. iApply (sem_typed_if _ [("n", _); ("fact", _)]);
+    set n := ("n", ℤ : sem_ty Σ).
+    set fact := ("fact", ℤ -{ stsig }-> () : sem_ty Σ).
+    rewrite /= -/n -/fact.
+    iApply (sem_typed_if _ [n; fact]);
       last (iApply sem_typed_sub_nil; 
             do 2 iApply sem_typed_weaken;
             iApply sem_typed_unit).
@@ -94,23 +99,23 @@ Section typing.
       iApply sem_typed_contraction; solve_sidecond.
       iApply sem_typed_bin_op; [constructor|iApply sem_typed_int|].
       iApply sem_typed_var. }
-    iApply sem_typed_seq.
-    - iApply sem_typed_contraction; solve_sidecond.
+    iApply (sem_typed_seq _ [n;fact]).
+    - iApply sem_typed_contraction; solve_copy.
       iApply sem_typed_frame_ms; first solve_copy.
       iApply sem_typed_swap_second.
       iApply sem_typed_frame_ms; first solve_copy.
-      iApply (sem_typed_app_ms _ _ []); first solve_sidecond.
+      iApply (sem_typed_app_ms _ [] _ _ _ ℤ); solve_sidecond.
       { iApply sem_typed_sub_nil. 
         iApply sem_typed_sub_ty; [iApply ty_le_u2aarr|].
         iApply sem_typed_val. iApply put_typed. }
       iApply sem_typed_bin_op; 
         [constructor| |iApply sem_typed_sub_nil;iApply sem_typed_var].
-      iApply sem_typed_app; first solve_sidecond; 
+      iApply (sem_typed_app_ms _ _ _ _ _ ()); solve_sidecond; 
         last (iApply sem_typed_sub_nil; iApply sem_typed_unit).
       iApply sem_typed_sub_nil; 
       iApply sem_typed_sub_ty; [iApply ty_le_u2aarr|].
       iApply sem_typed_val. iApply get_typed. 
-    - iApply (sem_typed_app _ [("fact", _)]); 
+    - iApply (sem_typed_app_ms _ [fact] _ _ _ ℤ); solve_copy;
         [iApply sem_typed_sub_ty; [iApply ty_le_u2aarr|];
          iApply sem_typed_sub_nil; iApply sem_typed_var|].
       iApply sem_typed_sub_nil.
@@ -128,24 +133,23 @@ Section typing.
     rewrite app_singletons.
     set A : sem_sig Σ → sem_ty Σ → sem_ty Σ := (λ _ _, () + ℤ)%T.
     set B : sem_sig Σ → sem_ty Σ → sem_ty Σ := (λ _ _, ℤ)%T.
-    iApply (sem_typed_deep_try _ [] _ _ "x" _ _ _ _ A B () _ ⊥ with "[] [] []"); solve_sidecond.
+    iApply (sem_typed_deep_try_os MS _ [] _ _ "x" _ _ _ _ A B () _ ⊥ with "[] [] []"); solve_sidecond.
     { rewrite /A /B -/stsig. 
-      iApply sem_typed_app; iApply sem_typed_sub_nil; 
-      last (iApply sem_typed_var).
+      iApply (sem_typed_app_ms _ [] _ _ _ ℤ); solve_copy; 
+      iApply sem_typed_sub_nil; last (iApply sem_typed_var).
       iApply sem_typed_sub_ty; [iApply ty_le_u2aarr|].
       iApply sem_typed_val. iApply fact_typed. }
     - iIntros (?). rewrite /A /B.
       iApply (sem_typed_match _ [("k", _); ("store", _)]); 
         solve_sidecond; [iApply sem_typed_var| |]; simpl.
-      + iApply sem_typed_app; [iApply sem_typed_var|].
+        + iApply sem_typed_app; [iApply sem_typed_var|].
         iApply (sem_typed_load_cpy _ _ _ _ ℤ); solve_sidecond.
         iApply sem_typed_swap_second. 
         iApply sem_typed_var.
       + iApply sem_typed_swap_third. iApply sem_typed_contraction; solve_sidecond.
         iApply sem_typed_swap_third.
         iApply (sem_typed_seq _ [("store", _); ("k", _)]). 
-        { iApply (sem_typed_store_cpy _ _ _ _ _ _ ℤ); 
-            solve_sidecond; iApply sem_typed_var. }
+        { iApply sem_typed_store_cpy; iApply sem_typed_var. }
         iApply sem_typed_app; [iApply sem_typed_var|].
         iApply (sem_typed_load_cpy _ _ _ _ ℤ); solve_sidecond.
         iApply sem_typed_var.
@@ -161,10 +165,10 @@ Section typing.
     set A : sem_sig Σ → sem_ty Σ → sem_ty Σ := (λ _ _, () + ℤ)%T.
     set B : sem_sig Σ → sem_ty Σ → sem_ty Σ := (λ _ _, ℤ)%T.
     rewrite - {1} (app_nil_r [("n", ℤ)]).
-    iApply (sem_typed_deep_try _ [] _ _ _ _ _ _ _ A B); solve_sidecond.
+    iApply (sem_typed_deep_try_os MS _ [] _ _ _ _ _ _ _ A B); solve_sidecond.
     { rewrite /A /B -/stsig. 
-      iApply sem_typed_app; iApply sem_typed_sub_nil; 
-      last (iApply sem_typed_var).
+      iApply (sem_typed_app_ms _ _ _ _ _ ℤ); solve_copy; 
+      iApply sem_typed_sub_nil; last iApply sem_typed_var.
       iApply sem_typed_sub_ty; [iApply ty_le_u2aarr|].
       iApply sem_typed_val. iApply fact_typed. }
     - iIntros (?). rewrite /A /B.
